Hashmap/List/BEq.lean
@@ -1,0 +1,15 @@
+/-
+Copyright (c) 2024 Lean FRO, LLC. All rights reserved.
+Released under Apache 2.0 license as described in the file LICENSE.
+Authors: Markus Himmel
+-/
+
+namespace List
+
+-- TODO
+@[simp] theorem nil_beq_cons [BEq α] {a : α} {as : List α} : ([] == a::as) = false := rfl
+@[simp] theorem nil_beq_nil [BEq α] : ([] : List α) == [] := rfl
+@[simp] theorem cons_beq_nil [BEq α] {a : α} {as : List α} : (a::as == []) = false := rfl
+@[simp] theorem cons_beq_cons [BEq α] {a b : α} {as bs : List α} : (a::as == b::bs) = ((a == b) && as == bs) := rfl
+
+end List
